internal/examples/semantics/interfaces.go
@@ -1,5 +1,9 @@
 package semantics
 
+// ----------------------------
+// SETUP
+// ----------------------------
+
 type geometryInterface interface {
 	Square() uint64
 	Volume() uint64
@@ -9,7 +13,11 @@ func measureSquare(t geometryInterface) uint64 {
 	return t.Square()
 }
 
-func measureVolume(t geometryInterface, e uint64, s string) uint64 {
+func measureVolumePlusN(t geometryInterface, n uint64) uint64 {
+	return t.Volume() + n
+}
+
+func measureVolume(t geometryInterface) uint64 {
 	return t.Volume()
 }
 
@@ -24,6 +32,10 @@ func (t SquareStruct) Square() uint64 {
 func (t SquareStruct) Volume() uint64 {
 	return t.Side * t.Side * t.Side
 }
+
+// ----------------------------
+// TESTS
+// ----------------------------
 
 func testBasicInterface() bool {
 	s := SquareStruct{
@@ -40,241 +52,38 @@ func testAssignInterface() bool {
 	return square == 9
 }
 
-func testParamsInterface() bool {
+func failing_testParamsInterface() bool {
 	s := SquareStruct{
 		Side: 3,
 	}
-	volume := measureVolume(s, 5, "string")
-	return volume == 32
+	volume := measureVolumePlusN(s, 1)
+	return volume == 28
 }
 
-// ----------------------------
-
-type bookInterface interface {
-	GetAuthor() string
-}
-
-type authorInterface interface {
-	GetBirthdate() uint64
-}
-
-type BookStruct struct {
-	Author string
-}
-
-type AuthorStruct struct {
-	Birthdate uint64
-}
-
-func (b BookStruct) GetAuthor() string {
-	return b.Author
-}
-
-func (a AuthorStruct) GetBirthdate() uint64 {
-	return a.Birthdate
-}
-
-func WhichAuthor(b bookInterface) string {
-	return b.GetAuthor()
-}
-
-func WhichBirthdate(a authorInterface) uint64 {
-	return a.GetBirthdate()
-}
-
-// Make sure mutliple interfaces are translated
-func multipleInterfacesTest() bool {
-	b := BookStruct{
-		Author: "Steve",
+func testMultipleInterface() bool {
+	s := SquareStruct{
+		Side: 3,
 	}
-	a := AuthorStruct{
-		Birthdate: 11011998,
-	}
-	return WhichAuthor(b) == "Steve" && WhichBirthdate(a) == 11011998
+	square1 := measureSquare(s)
+	square2 := measureSquare(s)
+	return square1 == square2
 }
 
-// Failing
-// func testEmptyInterface() bool {
-// 	var i interface{}
-// 	var j interface{}
-// 	return i == j
-// }
+func testBinaryExprInterface() bool {
+	s := SquareStruct{
+		Side: 3,
+	}
+	square1 := measureSquare(s)
+	square2 := measureVolume(s)
+	return square1 == measureSquare(s) && square2 == measureVolume(s)
+}
 
-// Failing
-// func testStringInterface() bool {
-// 	var i interface{} = "string"
-// 	var j interface{} = "string"
-// 	return i == j
-// }
-
-// func testTypeAssertionInterface() bool {
-// 	var i interface{} = NumStruct{3}
-
-// 	return i.(NumStruct) == NumStruct{3}
-// }
-
-// func testMultipleInterface() bool {
-// 	s := NumStruct{
-// 		Number: 3,
-// 	}
-// 	square1 := measureSquare(s)
-// 	square2 := measureSquare(s)
-
-// 	return square1 == square2
-// }
-
-// type shapeInterface interface {
-// 	describe() string
-// }
-
-// type polygonInterface interface {
-// 	sides() uint64
-// }
-
-// type shapeStruct struct {
-// 	Shape string
-// }
-
-// func (s shapeStruct) describe() string {
-// 	return s.Shape
-// }
-
-// type polygonStruct struct {
-// 	Shape string
-// 	Sides uint64
-// }
-
-// func (p polygonStruct) describe() string {
-// 	return p.Shape
-// }
-
-// func (p polygonStruct) sides() uint64 {
-// 	return p.Sides
-// }
-
-// func doublePointerInterfaceTest() bool {
-// 	s := shapeStruct{"circle"}
-// 	shapes := []shapeInterface{s, &s}
-
-// 	s.Shape = "square"
-
-// 	return shapes[0].describe() != shapes[1].describe()
-// }
-
-// func multipleFieldsInterfaceTest() bool {
-// 	s := polygonStruct{"triangle", 3}
-// 	return s.Shape == "triangle" && s.Sides == 3
-// }
-
-// type dogInterface interface {
-// 	Name() string
-// 	Speed() uint64
-// }
-
-// type catInterface interface {
-// 	Name() string
-// 	Weight() uint64
-// }
-
-// type Puppy string
-
-// func (p Puppy) Name() string {
-// 	return "Max"
-// }
-
-// func (p Puppy) Speed() uint64 {
-// 	return 1
-// }
-
-// type Kitten string
-
-// func (k Kitten) Name() string {
-// 	return "Max"
-// }
-
-// func (k Kitten) Weight() uint64 {
-// 	return 10
-// }
-
-// func sharedFunctionsInterfaceTest() bool {
-// 	var kit catInterface = Kitten("Kitten")
-// 	var pup dogInterface = Puppy("Puppy")
-// 	return pup.Name() == kit.Name()
-// }
-
-// type printInterface interface {
-// 	Assign(string)
-// 	GetTitle() string
-// }
-
-// type PaperStruct struct {
-// 	Title string
-// }
-
-// func (p *PaperStruct) Assign(t string) {
-// 	p.Title = t
-// }
-
-// func (p *PaperStruct) GetTitle() string {
-// 	return p.Title
-// }
-
-// func acceptAddressInterfaceTest() bool {
-// 	var p1 PaperStruct
-// 	var p2 PaperStruct
-// 	p1.Assign("Sample Title")
-// 	p2.Assign("Sample Title")
-// 	var print1 printInterface
-// 	var print2 printInterface
-// 	print1 = &p1
-// 	print2 = &p2
-// 	return print1.GetTitle() == print2.GetTitle()
-// }
-
-// type Flower interface {
-// 	Petals() uint64
-// }
-
-// type Flora interface {
-// 	Flower
-// 	Genus() string
-// }
-
-// type Lily struct{}
-
-// func (l Lily) Petals() uint64 { return 3 }
-// func (l Lily) Genus() string  { return "Lillium" }
-
-// type Rose struct{}
-
-// func (r Rose) Petals() uint64 { return 12 }
-// func (r Rose) Genus() string  { return "Rosa" }
-
-// type Daisy struct{}
-
-// func (d Daisy) Petals() uint64 { return 5 }
-// func (d Daisy) Genus() string  { return "Bellis" }
-
-// func polymorphismInterfaceTest() bool {
-// 	l := new(Lily)
-// 	r := new(Rose)
-// 	d := new(Daisy)
-// 	f := [...]Flower{l, r, d}
-// 	return f[0].Petals() == 3
-// }
-
-// func embeddingInterfaceTest() bool {
-// 	l := new(Lily)
-// 	r := new(Rose)
-// 	d := new(Daisy)
-// 	f := [...]Flora{l, r, d}
-// 	return f[0].Petals() == 3
-// }
-
-// func downcastInterfaceTest() bool {
-// 	l := Lily{}
-// 	var f Flora = l
-// 	return f.Petals() == f.(Flower).Petals()
-// }
-
-// slices, maps not supported
+func testIfStmtInterface() bool {
+	s := SquareStruct{
+		Side: 3,
+	}
+	if measureSquare(s) == 9 {
+		return true
+	}
+	return false
+}
